ROBINSON_PlusPlus/Meta.lean
@@ -67,5 +67,6 @@ import ROBINSON_PlusPlus.Meta.Delta0ReflectPrf
 import ROBINSON_PlusPlus.Meta.D3DottedPrf
 import ROBINSON_PlusPlus.Meta.EvalRunFnPrf
 import ROBINSON_PlusPlus.Meta.EvalNthcPrf
+import ROBINSON_PlusPlus.Meta.LineWFConsPrf
 import ROBINSON_PlusPlus.Meta.DiagonalTwo
 import ROBINSON_PlusPlus.Meta.GodelTwo
